examples/map/MapI.v
@@ -2,11 +2,11 @@ Require Import Coqlib ITreelib sflib.
 Require Import ImpPrelude.
 Require Import Events STS.
 Require Import Behavior.
-Require Import HMod.
+Require Import HMod PMod.
 Require Import Skeleton.
 Require Import MapHeader.
 Require Import PCM.
-Require Import STB IPM.
+Require Import STB IPM ITactics.
 
 
 Require Import sProp sWorld World SRF.
@@ -36,40 +36,42 @@ Section I.
   Local Open Scope string_scope.
   Context `{_W: CtxWD.t}.
   
-  Definition init: list val -> itree hmodE val :=
+  Definition init: list val -> itree pmodE val :=
     fun varg =>
       `sz: Z <- (pargs [Tint] varg)?;;
-      `r: val <- ccallU "alloc" [Vint sz];;
-      pput r;;;
-      _ <- (ITree.iter
-              (fun i =>
-                 if (Z_lt_le_dec i sz)
-                 then
-                   vptr <- (vadd r (Vint (i * 8)))?;;
-                   `r: val <- ccallU "store" [vptr; Vint 0];;
-                   Ret (inl (i + 1)%Z)
-                 else
-                   Ret (inr tt)) 0%Z);;
+      `hptr: val <- ccallU "alloc" [Vint sz];;
+      trigger (SPut "hptr" hptr↑);;;
+      (ITree.iter
+         (fun i =>
+            if (Z_lt_le_dec i sz)
+            then
+              vptr <- (vadd hptr (Vint (i * 8)))?;;
+              `_: val <- ccallU "store" [vptr; Vint 0];;
+              Ret (inl (i + 1)%Z)
+            else
+              Ret (inr tt)) 0%Z);;;
       Ret Vundef
   .
 
-  Definition get: list val -> itree hmodE val :=
+  Definition get: list val -> itree pmodE val :=
     fun varg =>
       k <- (pargs [Tint] varg)?;;
-      data <- trigger sGet;; data <- data↓?;; vptr <- (vadd data (Vint (k * 8)))?;;
+      hptr <- trigger (SGet "hptr");; hptr <- hptr↓?;;
+      vptr <- (vadd hptr (Vint (k * 8)))?;;
       `r: val <- ccallU "load" [vptr];; r <- (unint r)?;;
       Ret (Vint r)
   .
 
-  Definition set: list val -> itree hmodE val :=
+  Definition set: list val -> itree pmodE val :=
     fun varg =>
       '(k, v) <- (pargs [Tint; Tint] varg)?;;
-      data <- trigger sGet;; data <- data↓?;; vptr <- (vadd data (Vint (k * 8)))?;;
+      hptr <- trigger (SGet "hptr");; hptr <- hptr↓?;;
+      vptr <- (vadd hptr (Vint (k * 8)))?;;
       `_: val <- ccallU "store" [vptr; Vint v];;
       Ret Vundef
   .
 
-  Definition set_by_user: list val -> itree hmodE val :=
+  Definition set_by_user: list val -> itree pmodE val :=
     fun varg =>
       k <- (pargs [Tint] varg)?;;
       v <- trigger (IO "input" ([]: list Z));;
@@ -77,25 +79,25 @@ Section I.
   .
 
   Definition fnsems :=
-    [(MapName.init, cfunU init);
-     (MapName.get, cfunU get);
-     (MapName.set, cfunU set);
-     (MapName.set_by_user, cfunU set_by_user)].
+    [(MapName.init, (["hptr"], cfunU init));
+     (MapName.get,  (["hptr"], cfunU get));
+     (MapName.set,  (["hptr"], cfunU set));
+     (MapName.set_by_user, (["hptr"], cfunU set_by_user))].
   
-  Definition Sem: HModSem.t := {|
-    HModSem.fnsems := fnsems;
-    HModSem.initial_st := Vnullptr↑;
-    HModSem.initial_cond := True%I;
+  Program Definition Sem: PModSem.t := {|
+    PModSem.fnsems := fnsems;
+    PModSem.initial_st := [("hptr",tt↑)];
+  |}
+  .
+  Next Obligation. prove_scope. Qed.
+
+  Definition Mod: PMod.t := {|
+    PMod.get_modsem := fun _ => Sem;
+    PMod.sk := MapSK.t;
   |}
   .
 
-  Definition Mod: HMod.t := {|
-    HMod.get_modsem := fun _ => Sem;
-    HMod.sk := MapSK.t;
-  |}
-  .
-
-  Definition t := Seal.sealing "ccr" Mod.
+  Definition t: HMod.t := Seal.sealing "ccr" (PMod.to_hmod Mod).
 
 End I.
 End MapI.
