modules/SMod.v
@@ -8,6 +8,7 @@ Require Import PCM IPM.
 Require Import Events HMod.
 Require Export SMod2HMod.
 
+
 Set Implicit Arguments.
 
 Module SModSem.
@@ -17,18 +18,31 @@ Section SMODSEM.
   Variable stb: gname -> option fspec.
 
   Record t: Type := mk {
-    fnsems: list (gname * fspecbody);
-    initial_st: Any.t;
+    fnsems: alist gname (list string * fspecbody);
+    initial_st: alist string Any.t;
     initial_cond: iProp;
+    well_scoped:
+      forall fn k (IN: In k (fnsems_keys fn fnsems)), 
+          In k (List.map fst initial_st);
   }.
 
-  Definition transl (tr: fspecbody -> (Any.t -> itree hmodE Any.t)) (ms: t): HModSem.t := {|
-    HModSem.fnsems := List.map (fun '(fn, sb) => (fn, tr sb)) ms.(fnsems);
+  Lemma transl_well_scoped (ms: t): forall fn k,
+      In k (fnsems_keys (T:=Any.t -> itree hmodE Any.t) fn
+           (List.map (λ '(fn0, kv), (fn0, (fst kv, interp_sb_hp stb (snd kv)))) (fnsems ms)))
+    → In k (List.map fst (initial_st ms)).
+  Proof.
+    destruct ms. ss. i. unfold fnsems_keys in *.
+    rewrite alist_find_map in H. specialize (well_scoped0 fn k).
+    destruct (alist_find fn fnsems0); ss.
+    destruct p; ss. eauto.
+  Qed.
+
+  Definition to_hmod (ms: t): HModSem.t := {|
+    HModSem.fnsems := List.map (map_snd (λ ksb, (ksb.1, interp_sb_hp stb ksb.2))) ms.(fnsems);
     HModSem.initial_st := ms.(initial_st);
     HModSem.initial_cond := ms.(initial_cond);
+    HModSem.well_scoped := transl_well_scoped ms
   |}.
-
-  Definition to_hmod (ms: t): HModSem.t := transl (interp_sb_hp stb) ms.
 
 End SMODSEM.
 End SModSem.
@@ -45,15 +59,13 @@ Section SMOD.
     sk: Sk.t;
   }.
 
-  Definition transl (tr: Sk.t -> fspecbody -> ( Any.t -> itree hmodE Any.t)) (md: t): HMod.t := {|
-    HMod.get_modsem := fun sk => SModSem.transl (tr sk) (md.(get_modsem) sk);
+  Definition to_hmod (md:t): HMod.t := {|
+    HMod.get_modsem := fun sk => SModSem.to_hmod (stb sk) (md.(get_modsem) sk);
     HMod.sk := md.(sk);
-  |}.
-
-  Definition to_hmod (md:t): HMod.t := transl (fun sk => (interp_sb_hp (stb sk))) md.
+ |}.
     
-  Definition get_stb (mds: list t): Sk.t -> alist gname fspec :=
-    fun sk => List.map (map_snd fsb_fspec) (flat_map (SModSem.fnsems ∘ (flip get_modsem sk)) mds).
+  Definition get_stb (mds: list t): Sk.t -> alist gname (list string * fspec) :=
+    fun sk => List.map (map_snd (map_snd fsb_fspec)) (flat_map (SModSem.fnsems ∘ (flip get_modsem sk)) mds).
 
   Definition get_sk (mds: list t): Sk.t :=
     Sk.sort (fold_right Sk.add Sk.unit (List.map sk mds)).
