modules/PMod.v
@@ -1,0 +1,215 @@
+Require Import Coqlib.
+Require Import sflib.
+Require Import ITreelib.
+Require Import AList.
+Require Import Skeleton.
+Require Import Any.
+Require Import PCM IPM.
+Require Import Events HMod.
+
+Set Implicit Arguments.
+
+Module PModSem.
+Section PMODSEM.
+
+  Context `{Σ: GRA.t}.
+
+  Record t: Type := mk {
+    fnsems: alist gname (list string * (Any.t -> itree pmodE Any.t));
+    initial_st: alist string Any.t;
+    well_scoped:
+      forall fn k (IN: In k (fnsems_keys fn fnsems)), 
+          In k (List.map fst initial_st);
+  }.
+
+  Definition transl {R} (itr: itree pmodE R) : itree hmodE R
+    :=
+    translate inr1 itr.
+
+  Program Definition to_hmod (ms: t): HModSem.t := {|
+    HModSem.fnsems := List.map (map_snd (λ kb, (kb.1, (λ i, transl (kb.2 i))))) ms.(fnsems);
+    HModSem.initial_st := ms.(initial_st);
+    HModSem.initial_cond := emp;
+  |}.
+  Next Obligation.
+    destruct ms. s. ii.
+    eapply well_scoped0. instantiate (1:=fn).
+    unfold fnsems_keys, map_snd in *.
+    rewrite alist_find_map in H.
+    unfold o_map in *. des_ifs.
+  Qed.
+
+End PMODSEM.
+End PModSem.
+
+Module PMod.
+Section PMOD.
+
+  Context `{Σ: GRA.t}.
+
+  Record t: Type := mk {
+    get_modsem: Sk.t -> PModSem.t;
+    sk: Sk.t;
+  }.
+
+  Definition to_hmod (md:t): HMod.t := {|
+    HMod.get_modsem := fun sk => PModSem.to_hmod (md.(get_modsem) sk);
+    HMod.sk := md.(sk);
+ |}.
+    
+End PMOD.
+End PMod.
+
+Module PModRed.
+Section RED.
+
+  Context `{Σ: GRA.t}.
+
+(* itree reduction *)
+  Lemma transl_bind
+        (R S: Type)
+        (s : itree pmodE R) (k : R -> itree pmodE S)
+    :
+    PModSem.transl (s >>= k)
+    =
+    st <- PModSem.transl s;; PModSem.transl (k st).
+  Proof.
+    unfold PModSem.transl. rewrite (bisim_is_eq (translate_bind _ _ _)). eauto.
+  Qed.
+
+  Lemma transl_tau
+        (U: Type)
+        (t : itree _ U)
+    :
+      PModSem.transl (tau;; t)
+      =
+      tau;; (PModSem.transl t).
+  Proof.
+    unfold PModSem.transl. rewrite (bisim_is_eq (translate_tau _ _)). eauto.
+  Qed.
+
+  Lemma transl_ret
+        (U: Type)
+        (t: U)
+    :
+      PModSem.transl (Ret t)
+      =
+      Ret t.
+  Proof.
+    unfold PModSem.transl. rewrite (bisim_is_eq (translate_ret _ _)). eauto.
+  Qed.
+
+  Lemma transl_call
+        (R: Type)
+        (i: callE R)
+    :
+      PModSem.transl (trigger i)
+      =
+      trigger i.
+  Proof.
+    unfold PModSem.transl. unfold trigger.
+    rewrite (bisim_is_eq (translate_vis _ _ _ _)).
+    do 2 f_equal. extensionalities.
+    rewrite (bisim_is_eq (translate_ret _ _)). eauto.
+  Qed.
+
+  Lemma transl_pg
+        (R: Type)
+        (i: pgE R)
+    :
+      PModSem.transl (trigger i)
+      =
+      trigger i.
+  Proof.
+    unfold PModSem.transl. unfold trigger.
+    rewrite (bisim_is_eq (translate_vis _ _ _ _)).
+    do 2 f_equal. extensionalities.
+    rewrite (bisim_is_eq (translate_ret _ _)). eauto.
+  Qed.
+
+  Lemma transl_core
+        (R: Type)
+        (i: coreE R)
+    :
+      PModSem.transl (trigger i)
+      =
+      trigger i.
+  Proof.
+    unfold PModSem.transl. unfold trigger.
+    rewrite (bisim_is_eq (translate_vis _ _ _ _)).
+    do 2 f_equal. extensionalities.
+    rewrite (bisim_is_eq (translate_ret _ _)). eauto.
+  Qed.  
+
+(*  
+  Lemma transl_assume
+        P
+    : 
+      PModSem.transl (assume P)
+      =
+      assume P.
+  Proof.
+    rewrite /assume !transl_bind !transl_core !transl_ret. eauto.
+  Qed. 
+
+  Lemma transl_guarantee
+        P
+    : 
+      PModSem.transl (guarantee P)
+      =
+      guarantee P.
+  Proof.
+    rewrite /guarantee !transl_bind !transl_core !transl_ret. eauto.
+  Qed.
+
+  Lemma transl_triggerUB
+        (R: Type)
+    :
+      PModSem.transl (triggerUB)
+      =
+      triggerUB (A:=R).
+  Proof.
+    rewrite /triggerUB !transl_bind !transl_core.
+    f_equal; eauto. extensionalities. des_ifs.
+  Qed.  
+
+  Lemma transl_triggerNB
+        (R: Type)
+    :
+    PModSem.transl (triggerNB)
+    =
+    triggerNB (A:=R).
+  Proof.
+    rewrite /triggerNB !transl_bind !transl_core.
+    f_equal; eauto. extensionalities. des_ifs.
+  Qed.
+
+  Lemma transl_unwrapU 
+        (R: Type)
+        (i: option R)
+    :
+    PModSem.transl (@unwrapU pmodE _ _ i)
+    =
+    unwrapU i.
+  Proof.
+    rewrite /unwrapU. des_ifs.
+    - rewrite transl_ret; eauto.
+    - rewrite transl_triggerUB; eauto.
+  Qed.
+
+  Lemma transl_unwrapN
+        (R: Type)
+        (i: option R)
+    :
+      PModSem.transl (@unwrapN pmodE _ _ i)
+      =
+      unwrapN i.
+  Proof.
+    rewrite /unwrapN. des_ifs.
+    - rewrite transl_ret; eauto.
+    - rewrite transl_triggerNB; eauto.
+  Qed.
+ *)
+  
+End RED.
+End PModRed.
