simulations/isim/ISim.v
@@ -56,14 +56,14 @@ Section LEMMAS.
 
   (* Try to match bind pattern *)
   Lemma APC_start_clo Σ
-    I fls flt r g ps pt {R} RR st_src k_src sti_tgt  
+    fls flt I r g ps pt {R} RR st_src k_src sti_tgt  
     at_most o stb 
   :
-    @isim Σ I fls flt r g R RR true pt (st_src, _APC stb at_most o >>= (fun x => tau;; Ret x) >>= k_src) sti_tgt
+    @isim Σ fls flt I r g R RR true pt (st_src, _APC stb at_most o >>= (fun x => tau;; Ret x) >>= k_src) sti_tgt
   -∗  
-    @isim _ I fls flt r g R RR ps pt (st_src, interp_smodE_hmodE stb o (trigger APC) >>= k_src) sti_tgt.
+    @isim _ fls flt I r g R RR ps pt (st_src, interp_smod stb o (trigger APC) >>= k_src) sti_tgt.
   Proof.
-    unfold interp_smodE_hmodE. rewrite! interp_trigger. grind.
+    unfold interp_smod. rewrite! interp_trigger. grind.
     destruct sti_tgt. unfold HoareAPC.
     iIntros "K". 
     force_l. instantiate (1:= at_most).
@@ -71,12 +71,12 @@ Section LEMMAS.
   Qed.
 
   Lemma APC_stop_clo Σ
-    I fls flt r g ps pt {R} RR st_src k_src sti_tgt  
+    fls flt I r g ps pt {R} RR st_src k_src sti_tgt  
     at_most o stb
   :
-    @isim Σ I fls flt r g R RR true pt (st_src, k_src tt) sti_tgt
+    @isim Σ fls flt I r g R RR true pt (st_src, k_src tt) sti_tgt
   -∗  
-    @isim _ I fls flt r g R RR ps pt (st_src, _APC stb at_most o >>= (fun x => (tau;; Ret x) >>= k_src)) sti_tgt.
+    @isim _ fls flt I r g R RR ps pt (st_src, _APC stb at_most o >>= (fun x => (tau;; Ret x) >>= k_src)) sti_tgt.
   Proof.
     destruct sti_tgt.
     iIntros "K".
@@ -85,14 +85,14 @@ Section LEMMAS.
   Qed.
   
   Lemma APC_step_clo Σ
-    I fls flt r g ps pt {R} RR st_src k_src sti_tgt  
+    fls flt I r g ps pt {R} RR st_src k_src sti_tgt  
     at_most o stb next fn vargs fsp
     (SPEC: stb fn = Some fsp)
     (NEXT: (next < at_most)%ord)
   :
-    @isim Σ I fls flt r g R RR true pt (st_src, HoareCall true o fsp fn vargs >>= (fun _ => _APC stb next o) >>= (fun x => tau;; Ret x) >>= k_src) sti_tgt
+    @isim Σ fls flt I r g R RR true pt (st_src, HoareCall true o fsp fn vargs >>= (fun _ => _APC stb next o) >>= (fun x => tau;; Ret x) >>= k_src) sti_tgt
   -∗  
-    @isim _ I fls flt r g R RR ps pt (st_src, _APC stb at_most o >>= (fun x => (tau;; Ret x) >>= k_src)) sti_tgt.
+    @isim _ fls flt I r g R RR ps pt (st_src, _APC stb at_most o >>= (fun x => (tau;; Ret x) >>= k_src)) sti_tgt.
   Proof.
     destruct sti_tgt.
     iIntros "K". prep.
@@ -105,7 +105,7 @@ Section LEMMAS.
   Qed.
 
   Lemma hcall_clo Σ
-    I fls flt r g ps pt {R} RR st_src st_tgt k_src k_tgt
+    fls flt I r g ps pt {R} RR st_src st_tgt k_src k_tgt
     fn varg_src varg_tgt o X (x: shelve__ X) (D: X -> ord) P Q
     (* PURE, ... *)
     (ORD: ord_lt (D x) o)
@@ -115,9 +115,9 @@ Section LEMMAS.
       ∗ I st_src st_tgt 
       ∗ (∀st_src0 st_tgt0 vret_src vret_tgt, 
              (Q x vret_src vret_tgt ∗ I st_src0 st_tgt0) 
-          -∗ @isim Σ I fls flt r g R RR true true (st_src0, k_src vret_src) (st_tgt0, k_tgt vret_tgt)))
+          -∗ @isim Σ fls flt I r g R RR true true (st_src0, k_src vret_src) (st_tgt0, k_tgt vret_tgt)))
   -∗  
-    @isim _ I fls flt r g R RR ps pt (st_src, HoareCall true o (mk_fspec D P Q) fn varg_src >>= k_src) (st_tgt, trigger (Call fn varg_tgt) >>= k_tgt).
+    @isim _ fls flt I r g R RR ps pt (st_src, HoareCall true o (mk_fspec D P Q) fn varg_src >>= k_src) (st_tgt, trigger (Call fn varg_tgt) >>= k_tgt).
   Proof.
     iIntros "(P & IST & K)".
     unfold HoareCall. prep.
